\documentclass{article}
\usepackage{epsfig}
\pagestyle{empty}
\begin{document}
$ E = k'^T F k $
\pagebreak

$ T \leftarrow exp(\hat{\xi})T $
\pagebreak

$ \xi $
\pagebreak

$ TX_w $
\pagebreak

$Ji_{2\times3} = \frac{\partial [obs - \Pi(exp(\hat{\xi}) T X_w)]}{\partial X_w} $
\pagebreak

$Jj_{2\times6} = \frac{\partial [obs - \Pi(exp(\hat{\xi}) T X_w)]}{\partial \xi} $
\pagebreak

$ u = \frac{f_x X}{Z} + c_x $
\pagebreak

$ v = \frac{f_y Y}{Z} + c_v $
\pagebreak

$Ji_{3\times3} = \frac{\partial [obs - \Pi(exp(\hat{\xi}) T X_w)]}{\partial X_w} $
\pagebreak

$Jj_{3\times6} = \frac{\partial [obs - \Pi(exp(\hat{\xi}) T X_w)]}{\partial \xi} $
\pagebreak

$ ul = \frac{f_x X}{Z} + c_x $
\pagebreak

$ vl = \frac{f_y Y}{Z} + c_v $
\pagebreak

$ ur = \frac{f_x (X-b)}{Z} + c_x $
\pagebreak

$J_{2\times6}$
\pagebreak

$ = \frac{\partial [obs - \Pi(exp(\hat{\xi}) T X_w)]}{\partial \xi} $
\pagebreak

$J_{3\times6}$
\pagebreak

\end{document}
